

Advanced Engineering Mathematics

SERIES SOLUTIONS

Engr. Kaiveni Tom Dagcuta
Computer Engineering

1 Solutions About Ordinary Points

In this section, we introduce the **power series method** for solving linear differential equations near an *ordinary point*. This method is foundational in engineering mathematics and serves as a bridge between differential equations and special functions encountered in applied sciences.

Key Concept

An **ordinary point** of a differential equation is a point where all coefficient functions are analytic (i.e., can be expressed as power series).

1.1 General Form of the Differential Equation

We consider second-order linear differential equations of the form

$$p(x)y'' + q(x)y' + r(x)y = 0, \quad (1)$$

where $p(x)$, $q(x)$, and $r(x)$ are functions of x . At an ordinary point, the differential equation may be divided by $p(x)$, yielding

$$y'' + \frac{q(x)}{p(x)}y' + \frac{r(x)}{p(x)}y = 0. \quad (2)$$

Since $p(x_0) \neq 0$, the functions

$$\frac{q(x)}{p(x)}, \quad \frac{r(x)}{p(x)}$$

or

$$y'' + P(x)y' + Q(x)y = 0, \quad (3)$$

where

$$P(x) = \frac{q(x)}{p(x)}, \quad Q(x) = \frac{r(x)}{p(x)}.$$

Key Concept

A point $x = x_0$ is an **ordinary point** if both $P(x)$ and $Q(x)$ are analytic at x_0 .

Engineering Note

In practice, most equations with polynomial coefficients have ordinary points everywhere except where division by zero occurs.

1.2 Why Power Series Solutions Work

We know that:

- Analytic functions can be represented as power series.
- Power series can be differentiated and integrated term-by-term within their radius of convergence.

Hence, near an ordinary point x_0 , we may *assume* a solution of the form

$$y(x) = \sum_{n=0}^{\infty} a_n(x - x_0)^n. \quad (4)$$

This assumption is not a guess—it is justified by the theory of power series.

1.3 Derivatives of the Assumed Solution

Differentiating term-by-term,

$$y'(x) = \sum_{n=1}^{\infty} n a_n(x - x_0)^{n-1}, \quad (5)$$

$$y''(x) = \sum_{n=2}^{\infty} n(n-1) a_n(x - x_0)^{n-2}. \quad (6)$$

These expressions are substituted directly into the differential equation.

1.4 Method of Solution

The power series method about an ordinary point follows a systematic process:

1. Assume a power series solution centered at x_0 .
2. Compute y' and y'' .
3. Substitute into the differential equation.
4. Rewrite all terms using the same power of $(x - x_0)$.
5. Equate coefficients of like powers.
6. Obtain a **recurrence relation** for a_n .
7. Use initial conditions (if given) to find constants.

1.5 Example 1: Simple Ordinary Point

Example

Solve the differential equation

$$y'' - y = 0$$

about the ordinary point $x_0 = 0$ using a power series.

Step 1: Assume a power series solution

$$y = \sum_{n=0}^{\infty} a_n x^n.$$

Step 2: Compute derivatives

$$y' = \sum_{n=1}^{\infty} n a_n x^{n-1},$$
$$y'' = \sum_{n=2}^{\infty} n(n-1) a_n x^{n-2}.$$

Step 3: Substitute into the equation

$$\sum_{n=2}^{\infty} n(n-1) a_n x^{n-2} - \sum_{n=0}^{\infty} a_n x^n = 0.$$

Step 4: Align powers of x

Re-index the first sum by letting $n \rightarrow n+2$:

$$\sum_{n=0}^{\infty} (n+2)(n+1) a_{n+2} x^n - \sum_{n=0}^{\infty} a_n x^n = 0.$$

Step 5: Equate coefficients

$$(n+2)(n+1) a_{n+2} - a_n = 0.$$

Recurrence Relation:

$$a_{n+2} = \frac{a_n}{(n+2)(n+1)}.$$

1.6 Structure of the Solution

The recurrence relation shows that:

- Even-indexed coefficients depend only on a_0 .
- Odd-indexed coefficients depend only on a_1 .

Thus, the general solution is a linear combination of two power series:

$$y(x) = a_0 \left(1 + \frac{x^2}{2!} + \frac{x^4}{4!} + \cdots \right) + a_1 \left(x + \frac{x^3}{3!} + \frac{x^5}{5!} + \cdots \right).$$

Engineering Note

These series are recognized as the Maclaurin series for $\cosh x$ and $\sinh x$, respectively.

1.7 Example 2: Variable Coefficients with Ordinary Point

Example

Solve the differential equation

$$(1+x)y'' - xy' - y = 0$$

about $x_0 = 0$.

Since

$$p(x) = 1+x \quad \text{and} \quad p(0) = 1 \neq 0,$$

the point $x_0 = 0$ is an **ordinary point**. Hence, a power series solution about $x = 0$ exists.

Power Series Assumption

Assume a solution of the form

$$y(x) = \sum_{n=0}^{\infty} a_n x^n.$$

Then,

$$y'(x) = \sum_{n=1}^{\infty} n a_n x^{n-1}, \tag{7}$$

$$y''(x) = \sum_{n=2}^{\infty} n(n-1) a_n x^{n-2}. \tag{8}$$

Substitution into the Differential Equation

Substituting into

$$(1+x)y'' - xy' - y = 0,$$

we obtain

$$(1+x) \sum_{n=2}^{\infty} n(n-1)a_n x^{n-2} - x \sum_{n=1}^{\infty} n a_n x^{n-1} - \sum_{n=0}^{\infty} a_n x^n = 0.$$

Distributing terms,

$$\sum_{n=2}^{\infty} n(n-1)a_n x^{n-2} + \sum_{n=2}^{\infty} n(n-1)a_n x^{n-1} - \sum_{n=1}^{\infty} n a_n x^n - \sum_{n=0}^{\infty} a_n x^n = 0.$$

Reindexing the Series

Rewrite each sum in terms of x^n :

$$\sum_{n=0}^{\infty} (n+2)(n+1)a_{n+2}x^n + \sum_{n=1}^{\infty} n(n-1)a_n x^n - \sum_{n=1}^{\infty} n a_n x^n - \sum_{n=0}^{\infty} a_n x^n = 0.$$

Coefficient Comparison

For $n = 0$:

$$2a_2 - a_0 = 0 \quad \Rightarrow \quad a_2 = \frac{a_0}{2}.$$

For $n \geq 1$:

$$(n+2)(n+1)a_{n+2} + [n(n-1) - n - 1]a_n = 0.$$

Simplifying,

$$n(n-1) - n - 1 = n^2 - 2n - 1.$$

Thus, the recurrence relation is

$$a_{n+2} = \frac{2n+1-n^2}{(n+2)(n+1)} a_n, \quad n \geq 0.$$

Structure of the Solution

- Even-indexed coefficients depend only on a_0 .
- Odd-indexed coefficients depend only on a_1 .

Hence, the general solution about $x = 0$ is

$$y(x) = a_0 y_1(x) + a_1 y_2(x),$$

where y_1 and y_2 are linearly independent power series solutions.

Engineering Note

Variable-coefficient equations generally lead to non-terminating recurrence relations. Even when closed-form solutions do not exist, power series solutions remain valid within their radius of convergence.

1.8 Radius of Convergence

From Chapter 15:

- Power series solutions converge within a radius determined by the nearest singularity.
- The solution is guaranteed to be valid at least up to the closest point where $P(x)$ or $Q(x)$ becomes non-analytic.

Key Concept

For an ordinary point, the power series solution always exists and converges in some neighborhood of the point.

Summary

- Ordinary points allow direct application of power series methods.
- The method converts differential equations into algebraic recurrence relations.
- Solutions naturally connect to Taylor and Maclaurin series from Chapter 15.
- This technique forms the foundation for solving more complex equations near singular points.

2 POWER SERIES

2.1 Why Power Series Solutions Work

We know that:

- Analytic functions can be represented as power series.

- Power series can be differentiated and integrated term-by-term within their radius of convergence.

Hence, near an ordinary point x_0 , we may *assume* a solution of the form

$$y(x) = \sum_{n=0}^{\infty} a_n(x - x_0)^n. \quad (9)$$

This assumption is not a guess—it is justified by the theory of power series.

2.2 Derivatives of the Assumed Solution

Differentiating term-by-term,

$$y'(x) = \sum_{n=1}^{\infty} n a_n(x - x_0)^{n-1}, \quad (10)$$

$$y''(x) = \sum_{n=2}^{\infty} n(n-1) a_n(x - x_0)^{n-2}. \quad (11)$$

These expressions are substituted directly into the differential equation.

2.3 Method of Solution

The power series method about an ordinary point follows a systematic process:

1. Assume a power series solution centered at x_0 .
2. Compute y' and y'' .
3. Substitute into the differential equation.
4. Rewrite all terms using the same power of $(x - x_0)$.
5. Equate coefficients of like powers.
6. Obtain a **recurrence relation** for a_n .
7. Use initial conditions (if given) to find constants.

2.4 Example 1: Simple Ordinary Point

Example

Solve the differential equation

$$y'' - y = 0$$

about the ordinary point $x_0 = 0$ using a power series.

Step 1: Assume a power series solution

$$y = \sum_{n=0}^{\infty} a_n x^n.$$

Step 2: Compute derivatives

$$y' = \sum_{n=1}^{\infty} n a_n x^{n-1},$$
$$y'' = \sum_{n=2}^{\infty} n(n-1) a_n x^{n-2}.$$

Step 3: Substitute into the equation

$$\sum_{n=2}^{\infty} n(n-1) a_n x^{n-2} - \sum_{n=0}^{\infty} a_n x^n = 0.$$

Step 4: Align powers of x

Re-index the first sum by letting $n \rightarrow n+2$:

$$\sum_{n=0}^{\infty} (n+2)(n+1) a_{n+2} x^n - \sum_{n=0}^{\infty} a_n x^n = 0.$$

Step 5: Equate coefficients

$$(n+2)(n+1) a_{n+2} - a_n = 0.$$

Recurrence Relation:

$$a_{n+2} = \frac{a_n}{(n+2)(n+1)}.$$

2.5 Structure of the Solution

The recurrence relation shows that:

- Even-indexed coefficients depend only on a_0 .
- Odd-indexed coefficients depend only on a_1 .

Thus, the general solution is a linear combination of two power series:

$$y(x) = a_0 \left(1 + \frac{x^2}{2!} + \frac{x^4}{4!} + \cdots \right) + a_1 \left(x + \frac{x^3}{3!} + \frac{x^5}{5!} + \cdots \right).$$

Engineering Note

These series are recognized as the Maclaurin series for $\cosh x$ and $\sinh x$, respectively.

2.6 Example 2: Variable Coefficients with Ordinary Point

Example

Solve the differential equation

$$(1+x)y'' - xy' - y = 0$$

about $x_0 = 0$.

Since

$$p(x) = 1+x \quad \text{and} \quad p(0) = 1 \neq 0,$$

the point $x_0 = 0$ is an **ordinary point**. Hence, a power series solution about $x = 0$ exists.

Power Series Assumption

Assume a solution of the form

$$y(x) = \sum_{n=0}^{\infty} a_n x^n.$$

Then,

$$y'(x) = \sum_{n=1}^{\infty} n a_n x^{n-1}, \tag{12}$$

$$y''(x) = \sum_{n=2}^{\infty} n(n-1) a_n x^{n-2}. \tag{13}$$

Substitution into the Differential Equation

Substituting into

$$(1+x)y'' - xy' - y = 0,$$

we obtain

$$(1+x) \sum_{n=2}^{\infty} n(n-1)a_n x^{n-2} - x \sum_{n=1}^{\infty} n a_n x^{n-1} - \sum_{n=0}^{\infty} a_n x^n = 0.$$

Distributing terms,

$$\sum_{n=2}^{\infty} n(n-1)a_n x^{n-2} + \sum_{n=2}^{\infty} n(n-1)a_n x^{n-1} - \sum_{n=1}^{\infty} n a_n x^n - \sum_{n=0}^{\infty} a_n x^n = 0.$$

Reindexing the Series

Rewrite each sum in terms of x^n :

$$\sum_{n=0}^{\infty} (n+2)(n+1)a_{n+2}x^n + \sum_{n=1}^{\infty} n(n-1)a_n x^n - \sum_{n=1}^{\infty} n a_n x^n - \sum_{n=0}^{\infty} a_n x^n = 0.$$

Coefficient Comparison

For $n = 0$:

$$2a_2 - a_0 = 0 \quad \Rightarrow \quad a_2 = \frac{a_0}{2}.$$

For $n \geq 1$:

$$(n+2)(n+1)a_{n+2} + [n(n-1) - n - 1]a_n = 0.$$

Simplifying,

$$n(n-1) - n - 1 = n^2 - 2n - 1.$$

Thus, the recurrence relation is

$$a_{n+2} = \frac{2n+1-n^2}{(n+2)(n+1)} a_n, \quad n \geq 0.$$

Structure of the Solution

- Even-indexed coefficients depend only on a_0 .
- Odd-indexed coefficients depend only on a_1 .

Hence, the general solution about $x = 0$ is

$$y(x) = a_0 y_1(x) + a_1 y_2(x),$$

where y_1 and y_2 are linearly independent power series solutions.

Engineering Note

Variable-coefficient equations generally lead to non-terminating recurrence relations. Even when closed-form solutions do not exist, power series solutions remain valid within their radius of convergence.

2.7 Radius of Convergence

From Chapter 15:

- Power series solutions converge within a radius determined by the nearest singularity.
- The solution is guaranteed to be valid at least up to the closest point where $P(x)$ or $Q(x)$ becomes non-analytic.

Key Concept

For an ordinary point, the power series solution always exists and converges in some neighborhood of the point.

Summary

- Ordinary points allow direct application of power series methods.
- The method converts differential equations into algebraic recurrence relations.
- Solutions naturally connect to Taylor and Maclaurin series from Chapter 15.
- This technique forms the foundation for solving more complex equations near singular points.